created tutorial file

tutorial/Tut02.thy
@@ -23,13 +23,32 @@ lemma subst_lemma: "aval (subst x a' a) s = aval a (s(x := aval a' s))"
 lemma comp: "aval a1 s = aval a2 s \<Longrightarrow> aval (subst x a1 a) s = aval (subst x a2 a) s"
   apply(induction a arbitrary: x a1 a2 s) using subst_lemma by auto
 
+datatype aexp' = N' int | V' vname | Plus' aexp' aexp' | PI' vname
+
+
+fun aval' :: "aexp' \<Rightarrow> state \<Rightarrow> (val \<times> state)" where
+  "aval' (N' n) s = (n, s)" |
+  "aval' (V' v) s = (s v, s)" |
+  "aval' (Plus' i j) s = (case aval' i s of (i', s') \<Rightarrow>
+                        (case aval' j s' of (j', s'') \<Rightarrow> (i' + j', s'')))" |
+  "aval' (PI' v) s = (s v, s(v := (s v) + 1))"
 
 value "<>(x := 0)"
 value "aval' (Plus' (PI' ''x'') (V' ''x'')) <>"
 value "aval' (Plus' (Plus' (PI' ''x'') (PI' ''x'')) (PI' ''x'')) <>"
 
+lemma aval'_PI'_inc:
+  "aval' (PI' v) s = (r, s') \<Longrightarrow> s x \<le> s' x"
+  by auto
+
+lemma aval'_all_inc:
+  "aval' a s = (r, s') \<Longrightarrow> s x \<le> s' x"
+  apply(induction a arbitrary: x s)
+  apply(auto split: prod.splits) 
+
 lemma aval'_inc:
   "aval' a <> = (v, s') \<Longrightarrow> 0 \<le> s' x"
-  sorry
+  apply(induction a)
+  apply(auto simp: null_state_def split: prod.splits)
 
 end
